codelib/CodeLib/SepLogic/SmallStepTotalLifting.lean
@@ -1868,4 +1868,175 @@ theorem twp_swapElementsFunc3
     · rw [← show (1048568 : UInt32) + 4 = 1048572 from rfl]
       iexact Hlen
 
+theorem twp_subI64
+    {params localValues values : List Value}
+    {lhs rhs : UInt64} {code : Program} {arity : Nat}
+    {remainder : List Value} {controls : List ControlFrame}
+    {calls : List CallFrame} :
+    WP (.running
+      ⟨⟨params, localValues, .i64 (lhs - rhs) :: values⟩,
+        code, arity, remainder, controls, calls⟩ : Expr α) @ s; E
+        [{ Φ }] ⊢
+    WP (.running
+      ⟨⟨params, localValues, .i64 rhs :: .i64 lhs :: values⟩,
+        .subI64 :: code, arity, remainder, controls, calls⟩ : Expr α) @ s; E
+      [{ Φ }] :=
+  twp_pureStep _ _ _ (fun _ => Step.subI64)
+
+theorem twp_constI64
+    {params localValues values : List Value}
+    {value : UInt64} {code : Program} {arity : Nat}
+    {remainder : List Value} {controls : List ControlFrame}
+    {calls : List CallFrame} :
+    WP (.running
+      ⟨⟨params, localValues, .i64 value :: values⟩,
+        code, arity, remainder, controls, calls⟩ : Expr α) @ s; E
+        [{ Φ }] ⊢
+    WP (.running
+      ⟨⟨params, localValues, values⟩,
+        .constI64 value :: code, arity, remainder, controls, calls⟩ : Expr α) @ s; E
+      [{ Φ }] :=
+  twp_pureStep _ _ _ (fun _ => Step.constI64)
+
+theorem twp_orI64
+    {params localValues values : List Value}
+    {lhs rhs : UInt64} {code : Program} {arity : Nat}
+    {remainder : List Value} {controls : List ControlFrame}
+    {calls : List CallFrame} :
+    WP (.running
+      ⟨⟨params, localValues, .i64 (lhs ||| rhs) :: values⟩,
+        code, arity, remainder, controls, calls⟩ : Expr α) @ s; E
+        [{ Φ }] ⊢
+    WP (.running
+      ⟨⟨params, localValues, .i64 rhs :: .i64 lhs :: values⟩,
+        .orI64 :: code, arity, remainder, controls, calls⟩ : Expr α) @ s; E
+      [{ Φ }] :=
+  twp_pureStep _ _ _ (fun _ => Step.orI64)
+
+theorem twp_shlI64
+    {params localValues values : List Value}
+    {lhs rhs : UInt64} {code : Program} {arity : Nat}
+    {remainder : List Value} {controls : List ControlFrame}
+    {calls : List CallFrame} :
+    WP (.running
+      ⟨⟨params, localValues, .i64 (lhs <<< (rhs % 64)) :: values⟩,
+        code, arity, remainder, controls, calls⟩ : Expr α) @ s; E
+        [{ Φ }] ⊢
+    WP (.running
+      ⟨⟨params, localValues, .i64 rhs :: .i64 lhs :: values⟩,
+        .shlI64 :: code, arity, remainder, controls, calls⟩ : Expr α) @ s; E
+      [{ Φ }] :=
+  twp_pureStep _ _ _ (fun _ => Step.shlI64)
+
+theorem twp_shrUI64
+    {params localValues values : List Value}
+    {lhs rhs : UInt64} {code : Program} {arity : Nat}
+    {remainder : List Value} {controls : List ControlFrame}
+    {calls : List CallFrame} :
+    WP (.running
+      ⟨⟨params, localValues, .i64 (lhs >>> (rhs % 64)) :: values⟩,
+        code, arity, remainder, controls, calls⟩ : Expr α) @ s; E
+        [{ Φ }] ⊢
+    WP (.running
+      ⟨⟨params, localValues, .i64 rhs :: .i64 lhs :: values⟩,
+        .shrUI64 :: code, arity, remainder, controls, calls⟩ : Expr α) @ s; E
+      [{ Φ }] :=
+  twp_pureStep _ _ _ (fun _ => Step.shrUI64)
+
+theorem twp_ctzI64
+    {params localValues values : List Value}
+    {value : UInt64} {code : Program} {arity : Nat}
+    {remainder : List Value} {controls : List ControlFrame}
+    {calls : List CallFrame} :
+    WP (.running
+      ⟨⟨params, localValues,
+          .i64 (UInt64.ofNat (ctz64 64 value)) :: values⟩,
+        code, arity, remainder, controls, calls⟩ : Expr α) @ s; E
+        [{ Φ }] ⊢
+    WP (.running
+      ⟨⟨params, localValues, .i64 value :: values⟩,
+        .ctzI64 :: code, arity, remainder, controls, calls⟩ : Expr α) @ s; E
+      [{ Φ }] :=
+  twp_pureStep _ _ _ (fun _ => Step.ctzI64)
+
+theorem twp_wrapI64
+    {params localValues values : List Value}
+    {value : UInt64} {code : Program} {arity : Nat}
+    {remainder : List Value} {controls : List ControlFrame}
+    {calls : List CallFrame} :
+    WP (.running
+      ⟨⟨params, localValues,
+          .i32 (UInt32.ofNat (value.toNat % 2 ^ 32)) :: values⟩,
+        code, arity, remainder, controls, calls⟩ : Expr α) @ s; E
+        [{ Φ }] ⊢
+    WP (.running
+      ⟨⟨params, localValues, .i64 value :: values⟩,
+        .wrapI64 :: code, arity, remainder, controls, calls⟩ : Expr α) @ s; E
+      [{ Φ }] :=
+  twp_pureStep _ _ _ (fun _ => Step.wrapI64)
+
+theorem twp_extendUI32
+    {params localValues values : List Value}
+    {value : UInt32} {code : Program} {arity : Nat}
+    {remainder : List Value} {controls : List ControlFrame}
+    {calls : List CallFrame} :
+    WP (.running
+      ⟨⟨params, localValues, .i64 (UInt64.ofNat value.toNat) :: values⟩,
+        code, arity, remainder, controls, calls⟩ : Expr α) @ s; E
+        [{ Φ }] ⊢
+    WP (.running
+      ⟨⟨params, localValues, .i32 value :: values⟩,
+        .extendUI32 :: code, arity, remainder, controls, calls⟩ : Expr α) @ s; E
+      [{ Φ }] :=
+  twp_pureStep _ _ _ (fun _ => Step.extendUI32)
+
+theorem twp_eqI64
+    {params localValues values : List Value}
+    {lhs rhs : UInt64} {result : UInt32}
+    {code : Program} {arity : Nat}
+    {remainder : List Value} {controls : List ControlFrame}
+    {calls : List CallFrame}
+    (hresult : result = if lhs = rhs then 1 else 0) :
+    WP (.running
+      ⟨⟨params, localValues, .i32 result :: values⟩,
+        code, arity, remainder, controls, calls⟩ : Expr α) @ s; E
+        [{ Φ }] ⊢
+    WP (.running
+      ⟨⟨params, localValues, .i64 rhs :: .i64 lhs :: values⟩,
+        .eqI64 :: code, arity, remainder, controls, calls⟩ : Expr α) @ s; E
+      [{ Φ }] :=
+  twp_pureStep _ _ _ (fun _ => Step.eqI64 hresult)
+
+theorem twp_neI64
+    {params localValues values : List Value}
+    {lhs rhs : UInt64} {result : UInt32} {code : Program} {arity : Nat}
+    {remainder : List Value} {controls : List ControlFrame}
+    {calls : List CallFrame}
+    (hresult : result = if lhs ≠ rhs then 1 else 0) :
+    WP (.running
+      ⟨⟨params, localValues, .i32 result :: values⟩,
+        code, arity, remainder, controls, calls⟩ : Expr α) @ s; E
+        [{ Φ }] ⊢
+    WP (.running
+      ⟨⟨params, localValues, .i64 rhs :: .i64 lhs :: values⟩,
+        .neI64 :: code, arity, remainder, controls, calls⟩ : Expr α) @ s; E
+      [{ Φ }] :=
+  twp_pureStep _ _ _ (fun _ => Step.neI64 hresult)
+
+theorem twp_gtUI64
+    {params localValues values : List Value}
+    {lhs rhs : UInt64} {result : UInt32} {code : Program} {arity : Nat}
+    {remainder : List Value} {controls : List ControlFrame}
+    {calls : List CallFrame}
+    (hresult : result = if lhs > rhs then 1 else 0) :
+    WP (.running
+      ⟨⟨params, localValues, .i32 result :: values⟩,
+        code, arity, remainder, controls, calls⟩ : Expr α) @ s; E
+        [{ Φ }] ⊢
+    WP (.running
+      ⟨⟨params, localValues, .i64 rhs :: .i64 lhs :: values⟩,
+        .gtUI64 :: code, arity, remainder, controls, calls⟩ : Expr α) @ s; E
+      [{ Φ }] :=
+  twp_pureStep _ _ _ (fun _ => Step.gtUI64 hresult)
+
 end Wasm.SmallStep
